LambdaS5/coq/LjsPrettyInterm.v
@@ -1,4 +1,5 @@
 Set Implicit Arguments.
+Require Import LibInt.
 Require Import JsNumber.
 Require Import Utils.
 Require Import LjsShared.
@@ -236,5 +237,13 @@ Inductive eval_binary_op : binary_op -> store -> value -> value -> value -> Prop
     eval_binary_op binary_op_string_lt st (value_string s1) (value_string s2) (value_bool (string_lt s1 s2))
 | eval_binary_op_locale_compare : forall st s1 s2,
     eval_binary_op binary_op_locale_compare st (value_string s1) (value_string s2) (value_bool (string_lt s1 s2))
-(* TODO rest *)
+| eval_binary_op_is_accessor : forall st s ptr obj attrs,
+    binds st ptr obj -> 
+    object_property_is st obj s (Some attrs) ->
+    eval_binary_op binary_op_is_accessor st (value_object ptr) (value_string s) 
+        (value_bool (decide (is_accessor attrs)))
+| eval_binary_op_char_at : forall st s ch n,
+    0 <= to_int32 n -> String.get (abs (to_int32 n)) s = Some ch ->
+    eval_binary_op binary_op_char_at st (value_string s) (value_number n) 
+        (value_string (String ch EmptyString))
 .
