LambdaS5/coq/LjsRulesCorrectDefinitions.v
@@ -27,7 +27,6 @@ Include LjsPrettyRulesIndexedAux.
 Include LjsPrettyInterm.
 Include LjsStore.
 Include LjsAuxiliary.
-Include LjsOperators.
 Include LjsCommon.
 Include LjsValues.
 End L.
